examples/crypto/dh_hye/HyE.DH.fst
@@ -30,7 +30,7 @@ assume val dh_gen_key: unit -> St (dh_share*dh_exponent)
 type keysize = aeadKeySize AES_128_GCM
 type aes_key = lbytes keysize (* = b:bytes{B.length b = keysize} *)
 
-type log_t (i:id) (r:rid) = m_rref r (seq (PlainDH.key*dh_share)) grows
+type log_t (i:id) (r:rid) = m_rref r (seq (PlainDH.key*i:ae_id{b2t (ae_honest i)}*dh_share)) grows
 
 noeq type dh_pkey = 
   | DH_pkey:  #pk_i:id -> #region:rid ->rawpk:dh_share -> log:log_t pk_i region -> dh_pkey
@@ -38,9 +38,11 @@ noeq type dh_pkey =
 
 noeq abstract type dh_skey =
   | DH_skey: #sk_i:id -> rawsk:dh_exponent -> pk:dh_pkey -> dh_skey 
-  
 
-val keygen: #i:id -> (parent:rid) -> ST (dh_pair:dh_pkey * dh_skey)
+val getIndex: dh_skey -> Tot(id)
+let getIndex k = k.sk_i
+
+val keygen: #i:id -> (parent:rid) -> ST (dh_pair:(k:dh_pkey{k.pk_i=i}) * (k:dh_skey{k.sk_i=i}))
   (requires (fun h -> True))
   (ensures (fun h0 k h1 -> True
 //  let (pk,sk) = k in
@@ -70,33 +72,37 @@ type safe_log_append pk entry h0 h1 =
    If we prf_odh is true, the output of this function is random, if both 
    share and exponent are honest.
 *)
-val prf_odh_snd: dh_skey -> dh_pkey -> St (PlainDH.key)
+val prf_odh_snd: sk:dh_skey -> pk:dh_pkey -> ST (PlainDH.key)
+  ( requires (fun _ -> True))
+  ( ensures (fun _ k _ -> HyE.AE.getIndex k = (pk.pk_i, sk.sk_i)
+  ))
 let prf_odh_snd dh_snd_sk dh_rcv_pk =
   let pk_id = dh_rcv_pk.pk_i in
   let sk_id = dh_snd_sk.sk_i in
-  let i = generate_ae_id pk_id sk_id in
-  if honest pk_id && prf_odh then
+  let i = pk_id, sk_id in
+  if ae_honest i && prf_odh then
     let k' = PlainDH.keygen i dh_rcv_pk.region in
-    write_at_end dh_rcv_pk.log (k',dh_snd_sk.pk.rawpk);
+    write_at_end dh_rcv_pk.log (k',i,dh_snd_sk.pk.rawpk);
     k'
   else
     let real_k = dh_exponentiate dh_rcv_pk.rawpk dh_snd_sk.rawsk in
-    PlainDH.coerce_key i dh_rcv_pk.region real_k 
+    let k=PlainDH.coerce_key i dh_rcv_pk.region real_k in
+    k
 
 
-val prf_odh_rcv: #(sk_id:id) -> dh_share -> dh_skey -> St (PlainDH.key)
+val prf_odh_rcv: #(sk_id:id) -> dh_share -> dh_skey -> St (ae_id*PlainDH.key)
 let prf_odh_rcv #sk_id dh_sh dh_rcv_sk =
   if honest sk_id && prf_odh then
     let log = m_read dh_rcv_sk.pk.log in
-    let entry = seq_find (fun (k,dh_pk) -> dh_pk=dh_sh) log in
+    let entry = seq_find (fun (k,i,dh_pk) -> dh_pk=dh_sh) log in
     match entry with
-    | Some (k',_) -> k'
+    | Some (k',i,_) -> i,k'
     | None -> 
-      let i = generate_ae_id (dishonestId()) sk_id in
+      let i = (dishonestId()), sk_id in
       let raw_k = dh_exponentiate dh_sh dh_rcv_sk.rawsk in
-      PlainDH.coerce_key i dh_rcv_sk.pk.region raw_k
+      i, PlainDH.coerce_key i dh_rcv_sk.pk.region raw_k
   else
     let dis_id = dishonestId() in
-    let i = generate_ae_id dis_id sk_id in
+    let i = dis_id, sk_id in
     let raw_k = dh_exponentiate dh_sh dh_rcv_sk.rawsk in
-    PlainDH.coerce_key i dh_rcv_sk.pk.region raw_k
+    i,PlainDH.coerce_key i dh_rcv_sk.pk.region raw_k
