examples/crypto/dh_hye/HyE.HPKE.fst
@@ -33,7 +33,6 @@ open HyE.Indexing
 
 module B = Platform.Bytes
 
-
 type rid = FStar.Monotonic.Seq.rid
 
 (**
@@ -41,7 +40,7 @@ type rid = FStar.Monotonic.Seq.rid
    that is used for the encryption/decryption. The secret key is abstract.
 *)
 noeq abstract type hpke_pkey (pk_id:id) =
-  | PKey: #region:rid -> (dh_pk:dh_pkey)  -> hpke_pkey pk_id
+  | PKey: #region:rid -> dh_pk:dh_pkey{dh_pk.pk_i=pk_id} -> hpke_pkey pk_id
 
 noeq abstract type hpke_skey (sk_id:id) =
   | SKey: dh_sk:dh_skey -> hpke_pk:hpke_pkey sk_id -> hpke_skey sk_id
@@ -59,39 +58,47 @@ let keygen #i (parent:rid) =
 *)
 type c = DH.dh_share * AE.cipher //lbytes(PKE.ciphersize + AE.ciphersize)
 
+
 (**
    For every new message we encrypt, we generate a new id. If that
    id is honest (which is only possible if pke is idealized), then
    we encrypt the protected_hpke_plain. Else we strip it of its 
    protection and encrypt the plain representation.
 *)
-val encrypt: #(i:id) -> #(pk_id:id) -> #(m_id:id) -> hpke_pkey pk_id -> protected_hpke_plain m_id -> St c 
-let encrypt #i #pk_id #m_id pk p =
+val encrypt: #(i:id) -> hpke_pkey i -> protected_hpke_plain i -> St c 
+let encrypt #i pk p =
   let region = new_region pk.region in
-  let eph_dh_pk,eph_dh_sk = DH.keygen #i region in
+  let eph_i = createId () in
+  let eph_dh_pk,eph_dh_sk = DH.keygen #eph_i region in
   let k = prf_odh_snd eph_dh_sk pk.dh_pk in
+  let ae_i = AE.getIndex k in
+  assert (getIndex eph_dh_sk = snd ae_i);
+  assert (pk.dh_pk.pk_i = fst ae_i);
+  assert (getIndex eph_dh_sk = eph_i);
+  assert (pk.dh_pk.pk_i = i);
+  assert (ae_i = (i,eph_i));
   let p' = 
-    match hpke_ind_cca && honest i with
+    match hpke_ind_cca && ae_honest ae_i with
     | true -> p
     | false -> PlainHPKE.repr p
   in
-  let ae_m = ae_message_wrap p' in
+  let ae_m = ae_message_wrap #ae_i p' in
   //let dh_m = dh_message_wrap #pk.i eph_dh_pk.rawpk in
-  eph_dh_pk.rawpk,(AE.encrypt k ae_m)
+  eph_dh_pk.rawpk,(AE.encrypt #ae_i k ae_m)
 
 
 val decrypt: #(i:id) -> hpke_skey i -> c -> option (protected_hpke_plain i)
 let decrypt #i sk c =
   let (dh_sh,ae_c) = c in 
-  let k = AE.keygen sk.hpke_pk.region sk.dh_sk dh_sh in
+  let ae_i,k = prf_odh_rcv #i dh_sh sk.dh_sk in
   let hpke_p =
-    (match AE.decrypt k ae_c with
-    | Some p -> Some (PlainAE.ae_message_unwrap p)
+    (match AE.decrypt #ae_i k ae_c with
+    | Some p -> Some (PlainAE.ae_message_unwrap #ae_i p)
     | None -> None)
   in
   match hpke_p with
   | Some p' -> 
-    (if hpke_ind_cca && honest i then
+    (if ae_honest ae_i && hpke_ind_cca then
       Some p'
     else 
       Some (PlainHPKE.coerce p'))
