examples/crypto/dh_hye/HyE.PlainAE.fst
@@ -11,29 +11,33 @@ open Platform.Bytes
    If it is an honest message, it encapsulates a (protected) hpke payload.
    If it is not an honest message, it is plain bytes.
 *)
-type ae_plain_content (i:id) = (
-  if honest i && hpke_ind_cca then
-    protected_hpke_plain i
+
+type ae_plain_content (i:ae_id) = (
+  if ae_honest i && hpke_ind_cca then
+    protected_hpke_plain (fst i)
   else 
-    hpke_plain i
+    hpke_plain (fst i)
   )
 
-noeq abstract type protected_ae_plain (i:id)=
+noeq abstract type protected_ae_plain (i:ae_id)=
   | Protected_ae_plain: (p:ae_plain_content i) -> protected_ae_plain i
+
 
 type ae_plain = bytes
 
-val length: #i:id -> (protected_ae_plain i) -> Tot nat
+
+val length: #i:ae_id -> (protected_ae_plain i) -> Tot nat
 let length #i p = 
-  if honest i && hpke_ind_cca then
-    PlainHPKE.length #i p.p
+  if ae_honest i && hpke_ind_cca then
+    let pk_i = fst i in
+    PlainHPKE.length #pk_i p.p
   else
     length p.p
 
 (**
    Coerced messages can only be flagged as not honest.
 *)
-val coerce: #i:id -> p:ae_plain_content i{not ae_ind_cca || not (honest i)} -> Tot (protected_ae_plain i)
+val coerce: #i:ae_id -> p:ae_plain_content i{not ae_ind_cca || not (ae_honest i)} -> Tot (protected_ae_plain i)
 let coerce #i p = 
   Protected_ae_plain #i p
 
@@ -41,10 +45,10 @@ let coerce #i p =
    We allow a transition from protected_ae_plain to ae_plain only if either there is no
    idealization or if if the message is not honest.
 *)
-val repr: #i:id -> p:protected_ae_plain i{not ae_ind_cca || not (honest i)} -> Tot (ae_plain_content i)
+val repr: #i:ae_id -> p:protected_ae_plain i{not ae_ind_cca || not (ae_honest i)} -> Tot (ae_plain_content i)
 let repr #i p = 
-  if honest i && ae_ind_cca then
-    PlainHPKE.repr #i p.p 
+  if ae_honest i && ae_ind_cca then
+    PlainHPKE.repr #(fst i) p.p 
   else
     p.p
 
@@ -53,9 +57,9 @@ let repr #i p =
    passing it on to AE.encrypt. If AE is idealized and the payload is honest, then we 
    wrap the payload into our abstract type in good faith. If not, we coerce it.
 *)
-val ae_message_wrap: #i:id -> p:ae_plain_content i -> Tot (protected_ae_plain i)
+val ae_message_wrap: #i:ae_id -> p:ae_plain_content i -> Tot (protected_ae_plain i)
 let ae_message_wrap #i p =
-  if honest i && ae_ind_cca then
+  if ae_honest i && ae_ind_cca then
     Protected_ae_plain p
   else
     coerce p
@@ -66,9 +70,9 @@ let ae_message_wrap #i p =
    we strip it of its protection in good faith. Otherwise we break it down to its 
    byte representation using repr.
 *)
-val ae_message_unwrap: #i:id -> p:protected_ae_plain i -> Tot (ae_plain_content i)
+val ae_message_unwrap: #i:ae_id -> p:protected_ae_plain i -> Tot (ae_plain_content i)
 let ae_message_unwrap #i p =
-  if honest i && ae_ind_cca then
+  if ae_honest i && ae_ind_cca then
     p.p
   else 
     repr p
